WFLemmas.v
@@ -15,310 +15,6 @@ Require Import Subst.
 Require Import Tactics.
 Require Import Judge.
 
-Lemma subst_distr_pair :
-  forall (A B D R : Type) (SA : Subst A D R) (SB : Subst B D R) 
-         (θ : subst_t D R)  (x : A) (y : B),
-    subst θ (x, y) = (subst θ x, subst θ y).
-Proof.
-  auto.
-Qed.
-
-Lemma subst_distr_pair_cons :
-  forall (A B D R : Type) (SA : Subst A D R) (SB : Subst B D R) 
-         (θ : subst_t D R) (x : A) (y : B) (l : list (A * B)),
-    subst θ ((x, y) :: l) = ((subst θ x, subst θ y) :: subst θ l).
-Proof.
-  auto.
-Qed.
-
-Lemma subst_distr_cons :
-  forall (A D R : Type) (SA : Subst A D R)
-         (θ : subst_t D R) (x : A) (l : list A),
-    subst θ (x :: l) = (subst θ x :: subst θ l).
-Proof.
-  auto.
-Qed.
-
-Lemma fresh_var :
-  forall x t Γ,
-    var_not_in x Γ -> In (x,t) Γ -> False.
-Proof.
-  unfold var_not_in in *; pair_crush.
-Qed.
-
-Lemma var_not_in_exp :
-  forall x e Γ,
-    (x <> ν) -> var_not_in x Γ -> wf_expr Γ e -> (e <> (var_e x)).
-Proof.
-  intros x e Γ neq not_in wf_exp;
-  inversion wf_exp; crush' fresh_var fail.
-Qed.
-
-Ltac wf_freshvar exp :=
-  match goal with
-    | [ x:var, G:type_env, V:var_not_in ?x ?G, H: wf_expr ?G _ |- _ ] => 
-      let V1 := fresh "V"  in
-      set (V1 := V);
-      eapply var_not_in_exp with (e := exp) in V1
-   end.
-
-Lemma wf_type_prop : 
-  forall Γ ν τ φ,
-    wf_type Γ { ν : τ | φ } -> wf_prop Γ φ.
-Proof.
-  pair_crush' False wf_type.
-Qed.
-
-Lemma wf_expr_ty_expr :
-  forall Γ Ξ e T,
-    expr_type Γ Ξ e T -> 
-    wf_expr Γ e.
-Proof.
-  intros ? ? ? ? H.
-  dependent induction H.
-  + constructor.
-  + apply wf_var with { ν : τ | φ }. 
-    assumption.
-  + auto. 
-Qed.
- 
-Ltac invert_wf_expr :=
-  match goal with
-    | [ e1 : expr, e2 : expr, H : wf_expr _ (fun_e _ ?e1 ?e2) |- appcontext[?e1] ] =>
-      inversion H; crush
-    | [ e1 : expr, e2 : expr, H : wf_expr _ (fun_e _ ?e1 ?e2) |- appcontext[?e2] ] =>
-      inversion H; crush
-  end.
-
-Ltac break_wf_e := 
-  repeat constructor; 
-  unfold subst in *;
-  unfold subst_var_one in *;
-  simpl;
-  invert_wf_expr.
-
-Hint Unfold subst.
-Hint Unfold subst_var_one.
-
-Lemma wf_expr_subst :
-  forall Γ e x,
-    wf_expr Γ e -> var_in x Γ ->
-    wf_expr Γ (subst (subst_var_one ν x) e).
-Proof.
-  intros; unfold var_in in *; induction e; autounfold in *; simpl;
-  first [
-      break_wf_e
-    | match goal with
-        | [ |- context[eq_dec ?x ?v] ] => destruct (eq_dec x v); crush' wf_var fail
-        | _ => crush
-      end 
-    ].
-Qed.
-
-Lemma wf_prop_subst :
-  forall Γ φ x,
-    wf_prop Γ φ -> var_in x Γ ->
-    wf_prop Γ (subst (subst_var_one ν x) φ).
-Proof.
-  induction φ; intros; constructor; crush' wf_expr_subst ((wf_type, wf_prop), wf_expr).
-Qed.
-
-Lemma wf_not_in :
-  forall x t x' Γ,
-    var_not_in x' Γ -> wf_type Γ t -> (x,t) ∈ Γ ->
-    x <> x'.
-Proof.
-  intros; unfold var_not_in in *; crush; app_pair; crush.
-Qed.
-
-Lemma wf_expr_cons :
-  forall G e v t,
-         wf_expr G e -> wf_expr ((v,t) :: G) e.
-Proof.
-  intros.
-  induction H.
-  + constructor.
-  + apply in_cons with (a:=(v,t)) in H. apply wf_var with (t:=t0). assumption.
-  + constructor.
-  + constructor. apply IHwf_expr1. apply IHwf_expr2.
-Qed.
-
-Lemma wf_env_ty_cons :
-  forall G t v' t',
-    wf_type G t -> wf_type ((v',t') :: G) t.
-Proof.
-  intros.
-  inversion H. subst.
-  induction H0.
-  + constructor. constructor.
-  + constructor. constructor; apply wf_expr_cons; assumption.
-  + constructor. constructor. 
-    specialize (IHwf_prop (wf_reft_t Γ b p H0)). inversion IHwf_prop. subst. assumption.
-  + constructor. constructor.
-    inversion H. subst.
-    specialize (IHwf_prop1 (wf_reft_t Γ b p1 H0_)).
-    inversion IHwf_prop1. assumption. 
-    specialize (IHwf_prop2 (wf_reft_t Γ b p2 H0_0)).
-    inversion IHwf_prop2. assumption. 
-  + constructor. constructor.
-    inversion H. subst.
-    specialize (IHwf_prop1 (wf_reft_t Γ b p1 H0_)).
-    inversion IHwf_prop1. assumption.
-    specialize (IHwf_prop2 (wf_reft_t Γ b p2 H0_0)).
-    inversion IHwf_prop2. assumption. 
-Qed.
-  
-Lemma wf_env_ty :
-  forall G x t,
-    (x,t) ∈ G  -> wf_env G -> wf_type G t.
-Proof.
-  induction G as [ | [x' t']].
-  + intros. inversion H.
-  + intros. (* unfold In in H. destruct H. *)
-    apply in_inv in H.
-    destruct H.
-    inversion H.
-    subst.
-    inversion H0.
-    assumption.
-    apply wf_env_ty_cons.
-    apply IHG with (x:= x).
-    assumption.
-    inversion H0.
-    subst.
-    assumption.
-Qed.
-
-Lemma wf_env_cons_ty :
-  forall G x t,
-    wf_env ((x,t) :: G) -> wf_type ((x,t) :: G) t.
-Proof.
-  intros.
-  apply wf_env_ty with (x := x).
-  left. reflexivity.
-  assumption.
-Qed.
-
-Lemma wf_env_ty_binding :
-  forall G x b p,
-    wf_env G ->
-    (x, { ν : b | p }) ∈ G ->
-    wf_type G { ν : b | p }.
-Proof.
-  intros.
-  apply wf_env_ty with (x := x) (t := { ν : b | p }); assumption.
-Qed.
-
-Lemma wf_env_expr_ty :
-  forall G Grd e b p,
-    wf_env G ->
-    expr_type G Grd e { ν : b | p } -> 
-    wf_type G { ν : b | p }.
-Proof.
-  intros G Grd e b p wfenv etype.
-  inversion etype. 
-  + constructor; repeat constructor.
-  + subst. apply wf_env_ty_binding with (x := x) (b := b) (p := p) in wfenv; assumption.
-  + assumption.
-Qed.
-
-Lemma wf_env_nonmem :
-  forall x t G, (x,t) ∈ G -> wf_env G -> x <> ν.
-Proof.
-  induction G as [| [x' t']].
-  + intuition.
-  + intros InH WfH.
-    apply in_inv in InH.
-    inversion WfH. subst.
-    destruct InH. 
-    inversion H.
-    subst.
-    assumption.
-    apply IHG; assumption.
-Qed.
-
-Lemma wf_env_join :
-  forall  (X : guards) (G G' G'' : type_env),
-      join_env X G' G'' G -> wf_env G.
-Proof. 
-  intros. apply H.
-Qed.
-
-Lemma wf_heap_cons_env :
-  forall G H x t,
-    bind_not_in x H ->
-    wf_heap G H -> wf_heap ((x,t) :: G) H.
-Proof.
-  intros G H x t nomem wf.
-  induction H.
-  + constructor.
-  + inversion wf.
-    subst.
-    constructor; try assumption.
-    unfold bind_not_in in nomem.
-    rewrite Forall_forall in nomem.
-    unfold var_not_in.
-    rewrite Forall_forall.
-    intros [x' t'] [x'mem | x'mem].
-    inversion x'mem; subst.
-    specialize (nomem (l , (x0, t0))).
-    intro F.
-    apply nomem. left. reflexivity. simpl in F. simpl. congruence.
-    unfold var_not_in in H4.
-    rewrite Forall_forall in H4.
-    apply (H4 (x',t')). assumption.
-    apply wf_env_ty_cons. assumption.
-Qed.
-
-Ltac freshvar :=
-  match goal with 
-    | [ H : fresh ?v _ _ |- ?v <> ν ] =>
-      apply H
-    | [ H : fresh ?v _ _ |- var_not_in ?v _ ] =>
-      apply H
-    | [ H : fresh ?v _ _ |- bind_not_in ?v _ ] =>
-      apply H
-  end.
-    
-Ltac varin :=
-  try (assumption || congruence );
-  match goal with
-    | H : (?x, _) ∈ _ |- (?x, _) ∈ _ => eapply H
-    | H : (?x, _ ) ∈ ?G |- (?x, _) ∈ (_ :: ?G) =>
-      first [ right; varin | left; varin ]
-    | _ => idtac
-  end.
-
-Ltac wellformed_expr :=
-  try first [ constructor 
-            | eapply wf_var; try varin ].
-
-Ltac wellformed :=
-  match goal with
-    | |- wf_type _ _ => constructor; wellformed
-    | |- wf_prop _ _ => constructor; wellformed
-    | |- wf_expr _ _ => constructor; wellformed
-    | H : expr_type _ _ ?e _ |- wf_expr _ ?e => induction H; wellformed_expr
-  end.
-    
-Lemma wf_env_stmt :
-  forall P G G' H H' X s,
-    wf_env G ->
-    (P ; G ; H ; X) ⊢ s ::: (G' ; H') ->
-    wf_env G'.
-Proof.
-  intros P G G' H H' X s WF J.
-  induction J.
-  + assumption.
-  + assumption. 
-  + assumption.
-  + apply wf_env_var; try first [assumption | freshvar | wellformed];
-    apply IHexpr_type; assumption.
-  + apply wf_env_var; ( assumption || constructor || freshvar || wellformed ); constructor.
-  + eapply wf_env_join; eauto.
-  + auto.
-Qed.
-
 Ltac freshloc l :=
   destruct l;
   match goal with
@@ -353,14 +49,565 @@ Proof.
   firstorder.
 Qed.
 
+Lemma in_imp_var_in :
+  forall x t G,
+    (x,t) ∈ G -> var_in x G.
+Proof.
+  firstorder.
+Qed.
+
+Lemma var_in_cons :
+  forall a x G,
+    var_in x G -> var_in x (a :: G).
+Proof.
+  firstorder.
+Qed.
+
+Lemma var_not_in_cons :
+  forall a x G,
+    var_not_in x (a :: G) -> var_not_in x G.
+Proof.
+  unfold var_not_in.
+  intros.
+  rewrite Forall_forall in *.
+  firstorder.
+Qed.
+
+Lemma bind_in_cons :
+  forall a x H,
+    bind_in a H -> bind_in a (x :: H).
+Proof.
+  firstorder.
+Qed.
+
+Lemma bind_not_in_cons :
+  forall a x H,
+    bind_not_in x (a :: H) -> bind_not_in x H.
+Proof.
+  unfold bind_not_in.
+  intros.
+  rewrite Forall_forall in *.
+  firstorder.
+Qed.
+
+Lemma loc_not_in_cons :
+  forall a l H,
+    loc_not_in l (a :: H) -> loc_not_in l H.
+Proof.
+  intros. unfold loc_not_in in *. 
+  rewrite Forall_forall in *.
+  firstorder.
+Qed.
+
+Lemma fresh_loc_cons_1 :
+  forall x a G H,
+    fresh_loc x (a :: G) H -> fresh_loc x G H.
+Proof.
+  intros.
+  firstorder.
+  unfold fresh_loc in *. destruct x.
+  repeat split; try apply H0.
+  unfold fresh in H0.
+  eapply var_not_in_cons.
+  apply H0.
+Qed.
+
+Lemma fresh_loc_cons_2 :
+  forall x a G H,
+    fresh_loc x G (a :: H) -> fresh_loc x G H.
+Proof.
+  intros.
+  firstorder.
+  unfold fresh_loc in *. destruct x.
+  destruct H0 as [A [B C]].
+  repeat split; (eauto using bind_not_in_cons, 
+                             loc_not_in_cons, 
+                             fresh_imp_bind_not_in).
+  apply B.
+Qed.
+
+Lemma fresh_cons_1 :
+  forall x a G H,
+    fresh x G (a :: H) -> fresh x G H.
+Proof.
+  intros.
+  firstorder. eauto using bind_not_in_cons.
+Qed.
+
+Lemma fresh_cons_2 :
+  forall x a G H,
+    fresh x (a :: G) H -> fresh x G H.
+Proof.
+  intros.
+  firstorder. eauto using var_not_in_cons.
+Qed.
+
+Lemma wf_env_no_bind :
+  forall G H v t, 
+    wf_env H ((v, t) :: G) -> bind_not_in v H.
+Proof.
+  intros.
+  inversion H0. 
+  firstorder.
+Qed.
+
+Lemma fresh_var_neq :
+  forall G H v t x,
+    fresh x ((v,t) :: G) H -> 
+    x <> v.
+Proof.
+  unfold fresh.
+  intros.
+  intuition.
+  subst.
+  unfold var_not_in in *. rewrite Forall_forall in H0.
+  contradiction (H0 (v,t));
+  firstorder.
+Qed.
+
+Lemma var_neq_bind_not_in :
+  forall G H l x t v,
+    x <> v -> fresh v G H -> fresh v G ((l, (x,t)) :: H).
+Proof.
+  intros.
+  unfold fresh in *.
+  split; (repeat split); try apply H1.
+  unfold bind_not_in in *.
+  rewrite Forall_forall in *.
+  intros [l' [x' t']] [?|?]. 
+    inversion 0; subst; auto.
+    decompose [and or] H1.
+    eauto.
+Qed.
+
 Hint Resolve 
-     wf_env_ty_cons
-     wf_heap_cons_env
+     in_imp_var_in
+     var_in_cons
+     var_not_in_cons
+     bind_in_cons
+     bind_not_in_cons
+     fresh_loc_cons_1
+     fresh_loc_cons_2
+     fresh_cons_1
+     fresh_cons_2
      fresh_imp_loc_not_in
      fresh_imp_var_not_vv
      fresh_imp_var_not_in
      fresh_imp_bind_not_in
+     fresh_var_neq
+     var_neq_bind_not_in
+     wf_env_no_bind
 : wf.
+
+Lemma var_neq_fresh_loc :
+  forall G H x l t,
+    (V l) <> x -> 
+    fresh_loc (L l) G H -> fresh_loc (L l) ((x,t) :: G) H.
+Proof.
+  intros.
+  unfold fresh_loc in *.
+  decompose [and] H1.
+  repeat split; eauto with wf.
+  unfold fresh in H4.
+  decompose [and] H4.
+  unfold var_not_in in *. rewrite Forall_forall in *.
+  intros [x' t'] mem.
+  destruct mem. inversion H6. subst.
+    intuition.
+    auto.
+Qed.
+
+Hint Resolve var_neq_fresh_loc : wf.
+
+Hint Constructors
+     wf_type
+     wf_env
+: wf.
+
+Lemma subst_distr_pair :
+  forall (A B D R : Type) (SA : Subst A D R) (SB : Subst B D R) 
+         (θ : subst_t D R)  (x : A) (y : B),
+    subst θ (x, y) = (subst θ x, subst θ y).
+Proof.
+  auto.
+Qed.
+
+Lemma subst_distr_pair_cons :
+  forall (A B D R : Type) (SA : Subst A D R) (SB : Subst B D R) 
+         (θ : subst_t D R) (x : A) (y : B) (l : list (A * B)),
+    subst θ ((x, y) :: l) = ((subst θ x, subst θ y) :: subst θ l).
+Proof.
+  auto.
+Qed.
+
+Lemma subst_distr_cons :
+  forall (A D R : Type) (SA : Subst A D R)
+         (θ : subst_t D R) (x : A) (l : list A),
+    subst θ (x :: l) = (subst θ x :: subst θ l).
+Proof.
+  auto.
+Qed.
+
+Lemma fresh_var :
+  forall x t Γ,
+    var_not_in x Γ -> In (x,t) Γ -> False.
+Proof.
+  unfold var_not_in in *; pair_crush.
+Qed.
+
+(* Lemma var_not_in_exp : *)
+(*   forall x e Γ Σ, *)
+(*     (x <> ν) -> var_not_in x Γ -> wf_expr Γ Σ e -> (e <> (var_e x)). *)
+(* Proof. *)
+(*   intros x e Γ Σ neq not_in wf_exp. *)
+(*   inversion wf_exp. subst. *)
+(*   inversion wf_exp; crush' fresh_var fail. *)
+(* Qed. *)
+
+(* Ltac wf_freshvar exp := *)
+(*   match goal with *)
+(*     | [ x:var, G:type_env, V:var_not_in ?x ?G, H: wf_expr ?G _ |- _ ] =>  *)
+(*       let V1 := fresh "V"  in *)
+(*       set (V1 := V); *)
+(*       eapply var_not_in_exp with (e := exp) in V1 *)
+(*    end. *)
+
+Lemma wf_type_prop : 
+  forall Γ Σ ν τ φ,
+    wf_type Γ Σ { ν : τ | φ } -> wf_prop Γ Σ φ.
+Proof.
+  pair_crush' False wf_type.
+Qed.
+
+Hint Constructors wf_expr : wf.
+
+Lemma wf_expr_ty_expr :
+  forall Γ Σ Ξ e T,
+    expr_type Γ Σ Ξ e T -> 
+    wf_expr Γ Σ e.
+Proof.
+  intros ? ? ? ? ? H.
+  dependent induction H; eauto with wf.
+Qed.
+ 
+Ltac invert_wf_expr :=
+  match goal with
+    | [ e1 : expr, e2 : expr, H : wf_expr _ (fun_e _ ?e1 ?e2) |- appcontext[?e1] ] =>
+      inversion H; crush
+    | [ e1 : expr, e2 : expr, H : wf_expr _ (fun_e _ ?e1 ?e2) |- appcontext[?e2] ] =>
+      inversion H; crush
+  end.
+
+Ltac break_wf_e := 
+  repeat constructor; 
+  unfold subst in *;
+  unfold subst_var_one in *;
+  simpl;
+  invert_wf_expr.
+
+Hint Unfold subst.
+Hint Unfold subst_var_one.
+
+Lemma wf_expr_subst :
+  forall Γ Σ e x,
+    wf_expr Γ Σ e -> var_in x Γ ->
+    wf_expr Γ Σ (subst (subst_var_one ν x) e).
+Proof.
+  intros; unfold var_in in *; induction e; autounfold in *; simpl.
+  auto.
+  match goal with
+    | [ |- context[eq_dec ?x ?v] ] => destruct (eq_dec x v); crush' wf_var_ctx fail
+    | _ => crush
+  end.
+  constructor; eauto with wf;
+  inversion H; eauto.
+Qed.
+
+Lemma wf_prop_subst :
+  forall Γ Σ φ x,
+    wf_prop Γ Σ φ -> var_in x Γ ->
+    wf_prop Γ Σ (subst (subst_var_one ν x) φ).
+Proof.
+  induction φ; intros; constructor; crush' wf_expr_subst ((wf_type, wf_prop), wf_expr).
+Qed.
+
+Lemma wf_not_in :
+  forall x t x' Γ Σ ,
+    var_not_in x' Γ -> wf_type Γ Σ t -> (x,t) ∈ Γ ->
+    x <> x'.
+Proof.
+  intros; unfold var_not_in in *; crush; app_pair; crush.
+Qed.
+
+Lemma wf_expr_cons :
+  forall G Hp e v t,
+         wf_expr G Hp e -> wf_expr ((v,t) :: G) Hp e.
+Proof.
+  intros. induction H; eauto with wf.
+Qed.
+
+Lemma wf_expr_heap_cons :
+  forall G Hp e l v t,
+    wf_expr G Hp e -> wf_expr G ((l, (v, t)) :: Hp) e.
+Proof.
+  intros. induction H; eauto with wf.
+Qed.
+
+Hint Constructors wf_prop : wf.
+
+Lemma wf_env_ty_cons :
+  forall G Hp t v' t',
+    wf_type G Hp t -> wf_type ((v',t') :: G) Hp t.
+Proof.
+  intros.
+  inversion H. subst.
+  induction H0.
+  + eauto with wf.
+  + eauto using wf_expr_cons with wf. 
+  + constructor. constructor. 
+    specialize (IHwf_prop (wf_reft_t Γ Σ b p H0)). inversion IHwf_prop. subst. assumption.
+  + constructor. constructor.
+    inversion H. subst.
+    specialize (IHwf_prop1 (wf_reft_t Γ Σ b p1 H0_)).
+    inversion IHwf_prop1. assumption. 
+    specialize (IHwf_prop2 (wf_reft_t Γ Σ b p2 H0_0)).
+    inversion IHwf_prop2. assumption. 
+  + constructor. constructor.
+    inversion H. subst.
+    specialize (IHwf_prop1 (wf_reft_t Γ Σ b p1 H0_)).
+    inversion IHwf_prop1. assumption.
+    specialize (IHwf_prop2 (wf_reft_t Γ Σ b p2 H0_0)).
+    inversion IHwf_prop2. assumption. 
+Qed.
+  
+Hint Resolve wf_env_ty_cons : wf.
+
+Lemma wf_hp_ty_cons :
+  forall G Hp t l x t',
+    wf_type G Hp t ->
+    wf_type G ((l, (x,t')) :: Hp) t.
+Proof.
+  intros.
+  inversion H. subst.
+  induction H0.
+  + eauto with wf.
+  + eauto using wf_expr_heap_cons with wf.
+  + do 2 constructor.
+    specialize (IHwf_prop (wf_reft_t Γ Σ b p H0)). inversion IHwf_prop. subst. assumption.
+  + constructor. constructor.
+    inversion H. subst.
+    specialize (IHwf_prop1 (wf_reft_t Γ Σ b p1 H0_)).
+    inversion IHwf_prop1. assumption. 
+    specialize (IHwf_prop2 (wf_reft_t Γ Σ b p2 H0_0)).
+    inversion IHwf_prop2. assumption. 
+  + constructor. constructor.
+    inversion H. subst.
+    specialize (IHwf_prop1 (wf_reft_t Γ Σ b p1 H0_)).
+    inversion IHwf_prop1. assumption.
+    specialize (IHwf_prop2 (wf_reft_t Γ Σ b p2 H0_0)).
+    inversion IHwf_prop2. assumption. 
+Qed.
+
+Hint Resolve wf_hp_ty_cons : wf.
+
+Lemma wf_env_ty :
+  forall G Hp x t,
+    (x,t) ∈ G  -> wf_env Hp G -> wf_type G Hp t.
+Proof.
+  induction G as [ | [x' t']].
+  + intros. inversion H.
+  + intros. (* unfold In in H. destruct H. *)
+    apply in_inv in H.
+    destruct H.
+    inversion H.
+    subst.
+    inversion H0.
+    assumption.
+    apply wf_env_ty_cons.
+    apply IHG with (x:= x).
+    assumption.
+    inversion H0.
+    subst.
+    assumption.
+Qed.
+
+Lemma wf_env_cons_ty :
+  forall G H x t,
+    wf_env H ((x,t) :: G) -> wf_type ((x,t) :: G) H t.
+Proof.
+  intros.
+  apply wf_env_ty with (x := x); firstorder.
+Qed.
+
+Lemma wf_env_ty_binding :
+  forall G H x b p,
+    wf_env H G ->
+    (x, { ν : b | p }) ∈ G ->
+    wf_type G H { ν : b | p }.
+Proof.
+  intros.
+  apply wf_env_ty with (x := x) (t := { ν : b | p }); assumption.
+Qed.
+
+Lemma wf_env_expr_ty :
+  forall G H Grd e b p,
+    wf_env H G ->
+    expr_type G H Grd e { ν : b | p } -> 
+    wf_type G H { ν : b | p }.
+Proof.
+  intros G H Grd e b p wfenv etype.
+  inversion etype. 
+  + constructor. constructor. auto using wf_vv. constructor.
+  + eauto using wf_env_ty_binding.
+  + auto.
+Qed.
+
+Lemma wf_env_nonmem :
+  forall x t G Hp, (x,t) ∈ G -> wf_env Hp G -> x <> ν.
+Proof.
+  induction G as [| [x' t']].
+  + intuition.
+  + intros Hp InH WfH.
+    apply in_inv in InH.
+    inversion WfH. subst.
+    destruct InH. 
+    inversion H.
+    subst.
+    apply H3.
+    eauto.
+Qed.
+
+Lemma wf_env_join :
+  forall  (X : guards) Hp (G G' G'' : type_env),
+      join_env X Hp G' G'' G -> wf_env Hp G.
+Proof. 
+  intros. apply H.
+Qed.
+
+Ltac varneq :=
+  match goal with
+    | H : fresh _ _ _ |- _ <> _ =>
+      unfold fresh in H; decompose [and] H; varneq
+    | H : var_not_in _ _ |- _ <> _ =>
+      unfold var_not_in in H;
+        rewrite Forall_forall in H;
+        auto
+  end.
+
+Lemma wf_env_cons_hp :
+  forall G H x l t,
+  fresh x G H ->
+  fresh_loc l G H ->
+  (* H2 : wf_type Γ Σ t *)
+    wf_env H G -> wf_env ((l, (x,t)) :: H) G.
+Proof.
+  intros.
+  induction G.
+  + constructor.
+  + destruct a. 
+    inversion H2. subst.
+    apply wf_env_var;
+    eauto with wf.
+Qed.
+
+Lemma wf_heap_cons_env :
+  forall G H H0 x t,
+    bind_not_in x H0 ->
+    wf_heap G H H0 -> 
+    wf_heap ((x,t) :: G) H H0.
+Proof.
+  intros G H H0 x t nomem wf.
+  induction H0.
+  + constructor.
+  + inversion wf.
+    subst.
+    constructor; try assumption.
+    unfold bind_not_in in nomem.
+    rewrite Forall_forall in nomem.
+    repeat split. apply H3. 
+    unfold var_not_in. rewrite Forall_forall.
+    intros [x' t'] [x'mem | x'mem].
+    inversion x'mem; subst.
+    specialize (nomem (L l , (x0, t0))).
+    intro F.
+    apply nomem. left. reflexivity. simpl in F. simpl. congruence.
+    varneq.
+    eauto using IHlist with wf.
+    inversion wf. subst.
+    eapply var_neq_fresh_loc.
+    inversion wf. subst.
+    eauto with wf.
+    inversion wf. subst. unfold fresh_loc. destruct l.
+    inversion H12. split; auto.
+    split.
+    destruct H2.
+    eauto with wf.
+Qed.
+
+Hint Resolve wf_heap_cons_env : wf.
+
+Ltac freshvar :=
+  match goal with 
+    | [ H : fresh ?v _ _ |- ?v <> ν ] =>
+      apply H
+    | [ H : fresh ?v _ _ |- var_not_in ?v _ ] =>
+      apply H
+    | [ H : fresh ?v _ _ |- bind_not_in ?v _ ] =>
+      apply H
+  end.
+    
+Ltac varin :=
+  try (assumption || congruence );
+  match goal with
+    | H : (?x, _) ∈ _ |- (?x, _) ∈ _ => eapply H
+    | H : (?x, _ ) ∈ ?G |- (?x, _) ∈ (_ :: ?G) =>
+      first [ right; varin | left; varin ]
+    | _ => idtac
+  end.
+
+Ltac wellformed_expr :=
+  try first [ eauto with wf
+            | eapply wf_var_ctx; try varin 
+            | eapply wf_var_hp; try varin
+            ].
+
+Ltac wellformed :=
+  match goal with
+    | |- wf_type _ _ _ => constructor; wellformed
+    | |- wf_prop _ _ _ => constructor; wellformed
+    | |- wf_expr _ _ _ => constructor; wellformed
+    | H : expr_type _ _ _ ?e _ |- wf_expr _ _ _ => induction H; eauto with wf
+  end.
+    
+Lemma wf_env_stmt :
+  forall P G G' H H' X s,
+    wf_env H G ->
+    (P ; G ; H ; X) ⊢ s ::: (G' ; H') ->
+    wf_env H' G'.
+Proof.
+  intros P G G' H H' X s WF J.
+  induction J.
+  + assumption.
+  + assumption. 
+  + eauto using wf_env_cons_hp with wf.
+  + apply wf_env_var; eauto with wf.
+    wellformed.
+  + constructor; eauto with wf.
+    apply wf_env_cons_hp.
+    inversion H3.
+    unfold fresh. split; auto.
+    inversion H3.
+    unfold fresh_loc. split; eauto with wf. split; eauto with wf.
+    unfold fresh. split; eauto with wf.
+    inversion H3. subst. constructor. assumption. split; assumption.
+    inversion H3. subst. unfold fresh_loc. destruct l. split; try assumption.
+    eauto using wf_env_cons_hp with wf.
+  + apply wf_env_var; try first [assumption | freshvar | wellformed];
+    apply IHexpr_type; assumption.
+  + apply wf_env_var; ( assumption || constructor || freshvar || wellformed ); constructor.
+  + eapply wf_env_join; eauto.
+  + auto.
+Qed.
 
 (** Or should there just be a tactic...? **)
 
